dafny/src/lendingProtocol.dfy
@@ -3,6 +3,7 @@ include "util/number.dfy"
 include "util/maps.dfy"
 include "util/tx.dfy"
 include "fixed.dfy"
+include "erc20.dfy"
 
 
 import opened Number
@@ -21,82 +22,101 @@ class LendingProtocol {
     const baseRate: u256 := 20000000000000000
     const fixedAnnuBorrowRate: u256 := 300000000000000000
 
-    var usersCollateral: mapping<u160, u256>
-    var usersBorrowed: mapping<u160, u256>
+    var usersCollateral: mapping<u160, u256>  // ETH
+    var usersBorrowed: mapping<u160, u256>    // DAI
+    var usersBalances: mapping<u160, u256>    // DAI
 
     const WAD: u256 := 1000000000000000000
 
-    constructor() {
-        totalDeposit := 1000;
-        totalBorrow := 20;
+    var DAI: ERC20
+    var bDAI: ERC20
 
+    constructor() {
         usersCollateral := Map(map[], 0);
         usersBorrowed := Map(map[], 0);
+        usersBalances := Map(map[], 0);
+
+        DAI := new ERC20();
+        bDAI := new ERC20();
+    }
+
+    method bondAsset(msg: Transaction, amount: u256)
+    modifies this`totalDeposit
+    requires this.totalDeposit as nat + amount as nat <= MAX_U256 as nat {
+        // usersBalances := 
+        totalDeposit := totalDeposit + amount;
+    }
+    
+
+    method supply(msg: Transaction, amount: u256) returns (r: Result<()>)
+    modifies this`usersCollateral
+    requires amount as nat <= MAX_U256 - usersCollateral.Get(msg.sender) as nat {
+        usersCollateral := usersBalances.Set(msg.sender, usersCollateral.Get(msg.sender) + amount);
+        return Ok(());
+    }
+
+    method removeCollateral(msg: Transaction, amount: u256) returns (r: Result<()>)
+    modifies this`usersCollateral
+    requires amount as nat <= usersCollateral.Get(msg.sender) as nat {
+        usersCollateral := usersBalances.Set(msg.sender, usersCollateral.Get(msg.sender) - amount);
+        return Ok(());
     }
 
     method utilizationRatio() returns (utilizationRatio: u256)
-    // ensures utilizationRatio == this.totalBorrow / this.totalDeposit
     requires this.fixedAnnuBorrowRate > this.baseRate
-    requires this.totalBorrow as nat * (this.fixedAnnuBorrowRate - this.baseRate) as nat <= MAX_U256 as nat
+    requires this.totalBorrow as nat * WAD as nat <= MAX_U256 as nat
     requires this.totalDeposit != 0
     {
-        // var num: u256 := Sub(this.fixedAnnuBorrowRate, this.baseRate);
-        // var mul: u256 := Mul(this.totalBorrow, num);
-        // utilizationRatio := Fixed.Div(mul, this.totalDeposit);
-
-        var num: u256 := this.fixedAnnuBorrowRate - this.baseRate;
-        var mul: u256 := this.totalBorrow * num;
-        utilizationRatio := mul / this.totalDeposit;
+        var mul: u256 := Mul(this.totalBorrow, WAD);
+        utilizationRatio := Fixed.Div(mul, this.totalDeposit);
     }
 
     method interestMultiplier() returns (interestMul: u256)
     requires this.fixedAnnuBorrowRate > this.baseRate
-    requires this.totalBorrow as nat * (this.fixedAnnuBorrowRate - this.baseRate) as nat <= MAX_U256 as nat
+    requires this.totalBorrow as nat * WAD as nat <= MAX_U256 as nat
     requires this.totalDeposit != 0
     {
         var uRatio: u256 := utilizationRatio();
-        var num: u256 := this.fixedAnnuBorrowRate - this.baseRate;
+        var num: u256 := Sub(this.fixedAnnuBorrowRate, this.baseRate);
         if uRatio == 0 {
             interestMul := 0;
         }
         else {
-            interestMul := num / uRatio;
+            interestMul := Fixed.Div(num, uRatio);
         }
     }
     
 
     method borrowRate() returns (rate: u256)
     requires this.fixedAnnuBorrowRate > this.baseRate
-    requires this.totalBorrow as nat * (this.fixedAnnuBorrowRate - this.baseRate) as nat <= MAX_U256 as nat
+    requires this.totalBorrow as nat * WAD as nat <= MAX_U256 as nat
     requires this.totalDeposit != 0
-    ensures rate as nat <= MAX_U256 as nat
     {
         var uRatio: u256 := utilizationRatio();
         var interestMul: u256 := interestMultiplier();
         var product:u256 :=0;
         if uRatio as nat * interestMul as nat <= MAX_U256 as nat {
-            product := uRatio * interestMul;
+            product := Mul(uRatio, interestMul);
         }
         rate := 0;
         if product as nat + baseRate as nat <= MAX_U256 as nat {
-            rate := product + baseRate;
+            rate := Add(product, baseRate);
         }
     }
 
     method calculateBorrowFee(amount: u256) returns (fee: u256, paid: u256)
     requires this.fixedAnnuBorrowRate > this.baseRate
-    requires this.totalBorrow as nat * (this.fixedAnnuBorrowRate - this.baseRate) as nat <= MAX_U256 as nat
+    requires this.totalBorrow as nat * WAD as nat <= MAX_U256 as nat
     requires this.totalDeposit != 0
     {
         var borrowRate: u256 := borrowRate();
         fee := 0;
         if amount as nat * borrowRate as nat <= MAX_U256 as nat {
-            // fee := amount * borrowRate;
             fee := Mul(amount, borrowRate);
         }
         paid := 0;
         if amount as nat - fee as nat > 0 as nat {
-            paid := amount - fee;
+            paid := Sub(amount, fee);
         }
     }
 }
